Finished proof for (exp_to_fstar e) being equivalent to e and moved some cases of the proof into their own lemmas

rupicola/stlc_v2/RHC.fst
@@ -135,43 +135,52 @@ assume val lem_rel_beh (fs_e: wholeS) (e:wholeT) :
 
 // prove that this is equivalent for any fs_g
 // proof by induction on the expression (induction in backtranslation)
-val lem_exp_to_fstar g (e:exp) t (h:typing g e t) : Lemma 
-(equiv t (exp_to_fstar g e t h) e)
-let rec lem_exp_to_fstar g e t (h:typing g e t) =
-  assume(fv_in_env g e); 
-   match e with
-  | EUnit -> 
-    assert(forall b (s:gsub g b) (fsG:fs_env g).
-    fsG ∽ s ==> t ⦂ ((exp_to_fstar g EUnit t h) fsG, gsubst s EUnit)) 
+let exp_to_fstar_unit g
+  : Lemma 
+  (requires fv_in_env g EUnit)
+  (ensures equiv tunit (exp_to_fstar g EUnit tunit TyUnit) EUnit)
+  = assert (forall b (s:gsub g b) (fsG:fs_env g).
+           fsG ∽ s ==> tunit ⦂ ((exp_to_fstar g EUnit tunit TyUnit) fsG, gsubst s EUnit)) 
     by (explode ())
-  | ETrue -> 
-    assert(forall b (s:gsub g b) (fsG:fs_env g).
-    fsG ∽ s ==> t ⦂ ((exp_to_fstar g ETrue t h) fsG, gsubst s ETrue)) 
+
+let exp_to_fstar_true g
+  : Lemma
+  (requires fv_in_env g ETrue)
+  (ensures equiv tbool (exp_to_fstar g ETrue tbool TyTrue) ETrue)
+  = assert (forall b (s:gsub g b) (fsG:fs_env g).
+           fsG ∽ s ==> tbool ⦂ ((exp_to_fstar g ETrue tbool TyTrue) fsG, gsubst s ETrue)) 
     by (explode ())
-  | EFalse -> 
-    assert(forall b (s:gsub g b) (fsG:fs_env g).
-    fsG ∽ s ==> t ⦂ ((exp_to_fstar g EFalse t h) fsG, gsubst s EFalse)) 
+
+let exp_to_fstar_false g
+  : Lemma
+  (requires fv_in_env g EFalse)
+  (ensures equiv tbool (exp_to_fstar g EFalse tbool TyFalse) EFalse)
+  = assert (forall b (s:gsub g b) (fsG:fs_env g).
+           fsG ∽ s ==> tbool ⦂ ((exp_to_fstar g EFalse tbool TyFalse) fsG, gsubst s EFalse)) 
     by (explode ())
-  | EVar x ->
-    introduce forall b (s:gsub g b) fsG. fsG ∽ s ==> (Some?.v (g x)) ⦂ (get_v fsG x, gsubst s (EVar x)) with 
+
+let exp_to_fstar_var g (x:var{Some? (g x)}) h
+  : Lemma
+  (requires fv_in_env g (EVar x))
+  (ensures equiv (Some?.v (g x)) (exp_to_fstar g (EVar x) (Some?.v (g x)) h) (EVar x))
+  = 
+  introduce forall b (s:gsub g b) fsG. fsG ∽ s ==> (Some?.v (g x)) ⦂ (get_v fsG x, gsubst s (EVar x)) with 
+    begin
+    introduce _ ==> _ with _.
       begin
-      introduce _ ==> _ with _.
-        begin
-        assert (Some?.v (g x) ∋ (get_v fsG x, s x));
-        lem_values_are_expressions (Some?.v (g x)) (get_v fsG x) (s x)
-        end
+      assert (Some?.v (g x) ∋ (get_v fsG x, s x));
+      lem_values_are_expressions (Some?.v (g x)) (get_v fsG x) (s x)
       end
-   | EPair e1 e2 -> 
-    let TyPair #_ #_ #_ #t1 #t2 h1 h2 = h in
-    assume (fv_in_env g e1);
-    assume (fv_in_env g e2);
-    lem_exp_to_fstar g e1 t1 h1;
-    lem_exp_to_fstar g e2 t2 h2;
-    let t = mk_pair t1 t2 in
-    introduce forall b (s:gsub g b) fsG. fsG ∽ s ==> t ⦂ (((exp_to_fstar g e1 t1 h1) fsG, (exp_to_fstar g e2 t2 h2) fsG), gsubst s (EPair e1 e2)) with 
+    end
+
+let exp_to_fstar_pair g (t1 t2:typsr) (e1:exp) (e2:exp) fs_e1 fs_e2 : Lemma
+  (requires equiv t1 fs_e1 e1 /\ equiv t2 fs_e2 e2 /\ fv_in_env g (EPair e1 e2))
+  (ensures equiv (mk_pair t1 t2) (fun fsG -> (fs_e1 fsG, fs_e2 fsG)) (EPair e1 e2)) = 
+  let t = mk_pair t1 t2 in
+  introduce forall b (s:gsub g b) fsG. fsG ∽ s ==> t ⦂ ((fs_e1 fsG, fs_e2 fsG), gsubst s (EPair e1 e2)) with 
       begin
-      let fs_e1 = (exp_to_fstar g e1 t1 h1) fsG in
-      let fs_e2 = (exp_to_fstar g e2 t2 h2) fsG in
+      let fs_e1 = fs_e1 fsG in
+      let fs_e2 = fs_e2 fsG in
       let fs_e = (fs_e1, fs_e2) in
       let e = EPair (gsubst s e1) (gsubst s e2) in
       assert (gsubst s (EPair e1 e2) == e); 
@@ -189,25 +198,21 @@ let rec lem_exp_to_fstar g e t (h:typing g e t) =
               assert (t2 ∋ (fs_e2, e2'));
               assert (t ∋ (fs_e, EPair e1' e2'));
               lem_destruct_steps_epair e1' e2' e';
-              lem_values_are_expressions t fs_e (EPair e1' e2')
+              lem_values_are_expressions t fs_e (EPair e1' e2') // can turn this into e' - no?
             )
             end
           end
         end
       end
-  | EIf e1 e2 e3 ->
-    let TyIf #_ #_ #_ #_ #t h1 h2 h3 = h in
-    assume (fv_in_env g e1);
-    assume (fv_in_env g e2);
-    assume (fv_in_env g e3);
-    lem_exp_to_fstar g e1 tbool h1;
-    lem_exp_to_fstar g e2 t h2;
-    lem_exp_to_fstar g e3 t h3;
-    introduce forall b (s:gsub g b) fsG. fsG ∽ s ==> t ⦂ ((if (exp_to_fstar g e1 tbool h1) fsG then (exp_to_fstar g e2 t h2) fsG else (exp_to_fstar g e3 t h3) fsG), gsubst s (EIf e1 e2 e3)) with 
+
+let exp_to_fstar_if g (t:typsr) (e1:exp) (e2:exp) (e3:exp) fs_e1 fs_e2 fs_e3 : Lemma
+  (requires equiv tbool fs_e1 e1 /\ equiv t fs_e2 e2 /\ equiv t fs_e3 e3 /\ fv_in_env g (EIf e1 e2 e3))
+  (ensures equiv t (fun fsG -> if (fs_e1 fsG) then (fs_e2 fsG) else (fs_e3 fsG)) (EIf e1 e2 e3)) =
+  introduce forall b (s:gsub g b) fsG. fsG ∽ s ==> t ⦂ ((if (fs_e1 fsG) then (fs_e2 fsG) else (fs_e3 fsG)), gsubst s (EIf e1 e2 e3)) with 
       begin
-      let fs_e1 : bool = (exp_to_fstar g e1 tbool h1) fsG in
-      let fs_e2 : (get_Type t) = (exp_to_fstar g e2 t h2) fsG in
-      let fs_e3 : (get_Type t) = (exp_to_fstar g e3 t h3) fsG in
+      let fs_e1 : bool = fs_e1 fsG in
+      let fs_e2 : (get_Type t) = fs_e2 fsG in
+      let fs_e3 : (get_Type t) = fs_e3 fsG in
       let e = EIf (gsubst s e1) (gsubst s e2) (gsubst s e3) in
       assert (gsubst s (EIf e1 e2 e3) == e);
       let EIf e1 e2 e3 = e in
@@ -227,71 +232,199 @@ let rec lem_exp_to_fstar g e t (h:typing g e t) =
           end
         end
       end
-  (*| ELam body ->
-    let TyLam #_ #body #t1 #t2 hbody = h in
-    assume (fv_in_env (extend t1 g) body);
-    let g' = extend t1 g in
-    introduce forall b (s:gsub g b) fsG. fsG ∽ s ==> (mk_arrow t1 t2) ⦂ ((fun x -> (exp_to_fstar (extend t1 g) body t2 hbody)) (fs_stack fsG x)) fsG, gsubst s (ELam body)) with 
+
+let exp_to_fstar_fst g (t1 t2:typsr) (e12:exp) fs_e12 : Lemma
+  (requires equiv (mk_pair t1 t2) fs_e12 e12 /\ fv_in_env g (EFst e12))
+  (ensures equiv t1 (fun fsG -> fst #(get_Type t1) #(get_Type t2) (fs_e12 fsG)) (EFst e12)) =
+  introduce forall b (s:gsub g b) fsG. fsG ∽ s ==> t1 ⦂ (fst #(get_Type t1) #(get_Type t2) (fs_e12 fsG), gsubst s (EFst e12)) with
       begin
-      ()
-      end*)
-  (*| EApp e1 e2 ->
-    let TyApp #_ #_ #_ #t1 #t2 h1 h2 = h in
-    assume (fv_in_env g e1);
-    assume (fv_in_env g e2);
-    lem_exp_to_fstar g e1 (mk_arrow t1 t2) h1;
-    lem_exp_to_fstar g e2 t1 h2;
-    introduce forall b (s:gsub g b) fsG. fsG ∽ s ==> t2 ⦂ (((exp_to_fstar g e1 (mk_arrow t1 t2) h1) fsG) ((exp_to_fstar g e2 t1 h2) fsG), gsubst s (EApp e1 e2)) with
-      begin
-      let fs_e1 = (exp_to_fstar g e1 (mk_arrow t1 t2) h1) fsG in
-      let fs_e2 = (exp_to_fstar g e2 t1 h2) fsG in
-      let fs_e = fs_e1 fs_e2 in
-      let e = EApp (gsubst s e1) (gsubst s e2) in
-      assert (gsubst s (EApp e1 e2) == e);
-      let EApp e1 e2 = e in
-      introduce fsG ∽ s ==>  t2 ⦂ (fs_e, e) with _. 
+      let fs_e12 = fs_e12 fsG in
+      let fs_e = fst #(get_Type t1) #(get_Type t2) fs_e12 in
+      let e = EFst (gsubst s e12) in
+      assert (gsubst s (EFst e12) == e);
+      let EFst e12 = e in
+      introduce fsG ∽ s ==> t1 ⦂ (fs_e, e) with _. 
         begin
-        introduce forall (e':closed_exp). steps e e' /\ irred e' ==> t2 ∋ (fs_e, e') with
+        introduce forall (e':closed_exp). steps e e' /\ irred e' ==> t1 ∋ (fs_e, e') with
           begin
-          introduce _ ==> t2 ∋ (fs_e, e') with h. 
+          introduce _ ==> t1 ∋ (fs_e, e') with h. 
             begin
-              let steps_e_e' : squash (steps e e') = () in
-              FStar.Squash.map_squash #_ #(squash (t2 ∋ (fs_e, e'))) steps_e_e' (fun steps_e_e' ->
-                let (e11, e2') = destruct_steps_eapp e1 e2 e' steps_e_e' in
-                assert (mk_arrow t1 t2 ∋ (fs_e1, ELam e11));
-                ()
-              )
-            end
-          end
-        end
-      end*)
-  | EFst e ->
-    let TyFst #_ #_ #t1 #t2 h1 = h in
-    assume (fv_in_env g e);
-    lem_exp_to_fstar g e (mk_pair t1 t2) h1;
-    introduce forall b (s:gsub g b) fsG. fsG ∽ s ==> t1 ⦂ (fst #(get_Type t1) #(get_Type t2) ((exp_to_fstar g e (mk_pair t1 t2) h1) fsG), gsubst s (EFst e)) with
-      begin
-      let fs_e = (exp_to_fstar g e (mk_pair t1 t2) h1) fsG in
-      let fs_fe = fst #(get_Type t1) #(get_Type t2) fs_e in
-      let fe = EFst (gsubst s e) in
-      assert (gsubst s (EFst e) == fe);
-      let EFst e = fe in
-      introduce fsG ∽ s ==> t1 ⦂ (fs_fe, fe) with _. 
-        begin
-        introduce forall (fe':closed_exp). steps fe fe' /\ irred fe' ==> t1 ∋ (fs_fe, fe') with
-          begin
-          introduce _ ==> t1 ∋ (fs_fe, fe') with h. 
-            begin
-            let steps_fe_fe' : squash (steps fe fe') = () in
-            FStar.Squash.map_squash #_ #(squash (t1 ∋ (fs_fe, fe'))) steps_fe_fe' (fun steps_fe_fe' -> 
-              let e12' = destruct_steps_epair_fst e fe' steps_fe_fe' in
-              admit ()
+            let steps_e_e' : squash (steps e e') = () in
+            FStar.Squash.map_squash #_ #(squash (t1 ∋ (fs_e, e'))) steps_e_e' (fun steps_e_e' -> 
+              let e12' = destruct_steps_epair_fst e12 e' steps_e_e' in
+              eliminate (mk_pair t1 t2) ⦂ (fs_e12, e12) /\ steps e12 e12' /\ irred e12'
+              returns (mk_pair t1 t2) ∋ (fs_e12, e12') with _ _. ();
+              let EPair e1' e2' = e12' in
+              assert (t1 ∋ (fs_e, e1'));
+              lem_destruct_steps_epair_fst e1' e2' e';
+              assert (t1 ∋ (fs_e, e'))
               ) 
             end
           end
         end
       end
+
+let exp_to_fstar_snd g (t1 t2:typsr) (e12:exp) fs_e12 : Lemma
+  (requires equiv (mk_pair t1 t2) fs_e12 e12 /\ fv_in_env g (ESnd e12))
+  (ensures equiv t2 (fun fsG -> snd #(get_Type t1) #(get_Type t2) (fs_e12 fsG)) (ESnd e12)) =
+      introduce forall b (s:gsub g b) fsG. fsG ∽ s ==> t2 ⦂ (snd #(get_Type t1) #(get_Type t2) (fs_e12 fsG), gsubst s (ESnd e12)) with
+      begin
+      let fs_e12 = fs_e12 fsG in
+      let fs_e = snd #(get_Type t1) #(get_Type t2) fs_e12 in
+      let e = ESnd (gsubst s e12) in
+      assert (gsubst s (ESnd e12) == e);
+      let ESnd e12 = e in
+      introduce fsG ∽ s ==> t2 ⦂ (fs_e, e) with _. 
+        begin
+        introduce forall (e':closed_exp). steps e e' /\ irred e' ==> t2 ∋ (fs_e, e') with
+          begin
+          introduce _ ==> t2 ∋ (fs_e, e') with h. 
+            begin
+            let steps_e_e' : squash (steps e e') = () in
+            FStar.Squash.map_squash #_ #(squash (t2 ∋ (fs_e, e'))) steps_e_e' (fun steps_e_e' ->
+              let e12' = destruct_steps_epair_snd e12 e' steps_e_e' in
+              eliminate (mk_pair t1 t2) ⦂ (fs_e12, e12) /\ steps e12 e12' /\ irred e12'
+              returns (mk_pair t1 t2) ∋ (fs_e12, e12') with _ _. ();
+              let EPair e1' e2' = e12' in
+              assert (t2 ∋ (fs_e, e2'));
+              lem_destruct_steps_epair_snd e1' e2' e';
+              assert (t2 ∋ (fs_e, e'))
+              )
+            end
+          end
+        end
+      end
+
+let exp_to_fstar_app g (t1 t2:typsr) (e1:exp) (e2:exp) fs_e1 fs_e2 : Lemma
+  (requires equiv (mk_arrow t1 t2) fs_e1 e1 /\ equiv t1 fs_e2 e2 /\ fv_in_env g (EApp e1 e2))
+  (ensures equiv t2 (fun fsG -> (fs_e1 fsG) (fs_e2 fsG)) (EApp e1 e2)) = 
+    introduce forall b (s:gsub g b) fsG. fsG ∽ s ==> t2 ⦂ (((fs_e1 fsG) (fs_e2 fsG)), gsubst s (EApp e1 e2)) with
+      begin
+      let fs_e1 = fs_e1 fsG in
+      let fs_e2 = fs_e2 fsG in
+      let fs_e = fs_e1 fs_e2 in
+      let e = EApp (gsubst s e1) (gsubst s e2) in
+      assert (gsubst s (EApp e1 e2) == e);
+      let EApp e1 e2 = e in
+      introduce fsG ∽ s ==> t2 ⦂ (fs_e, e) with _.
+        begin
+        introduce forall (e':closed_exp). steps e e' /\ irred e' ==> t2 ∋ (fs_e, e') with
+          begin
+          introduce _ ==> t2 ∋ (fs_e, e') with h.
+            begin
+            let steps_e_e' : squash (steps e e') = () in
+            FStar.Squash.map_squash #_ #(squash (t2 ∋ (fs_e, e'))) steps_e_e' (fun steps_e_e' -> 
+              let (e11, e2') = destruct_steps_eapp e1 e2 e' steps_e_e' in
+              assert (t1 ∋ (fs_e2, e2'));
+              assert (irred (ELam e11));
+              introduce True ==> t1 ∋ (fs_e2, e2') with _.
+                begin
+                assert (t1 ⦂ (fs_e2, e2));
+                assert (steps e2 e2');
+                assert (irred e2')
+              end;
+              eliminate forall (v:value) (fs_v:get_Type t1). t1 ∋ (fs_v, v) ==> 
+                t2 ⦂ (fs_e1 fs_v, subst_beta v e11)
+              with e2' fs_e2;
+              assert (t2 ⦂ (fs_e, subst_beta e2' e11));
+              assert (mk_arrow t1 t2 ∋ (fs_e1, ELam e11));
+              assert (t2 ∋ (fs_e, e'))
+              )
+            end
+          end
+        end
+      end
+  
+
+val lem_exp_to_fstar g (e:exp) t (h:typing g e t) : Lemma 
+(equiv t (exp_to_fstar g e t h) e)
+let rec lem_exp_to_fstar g e t (h:typing g e t) =
+  assume(fv_in_env g e); 
+   match e with
+  | EUnit -> exp_to_fstar_unit g
+  | ETrue -> exp_to_fstar_true g
+  | EFalse -> exp_to_fstar_false g
+  | EVar x -> exp_to_fstar_var g x h
+  | EPair e1 e2 -> 
+    let TyPair #_ #_ #_ #t1 #t2 h1 h2 = h in
+    assume (fv_in_env g e1);
+    assume (fv_in_env g e2);
+    lem_exp_to_fstar g e1 t1 h1;
+    lem_exp_to_fstar g e2 t2 h2;
+    let fs_e1 = (exp_to_fstar g e1 t1 h1) in
+    let fs_e2 = (exp_to_fstar g e2 t2 h2) in
+    exp_to_fstar_pair g t1 t2 e1 e2 fs_e1 fs_e2
+  | EIf e1 e2 e3 ->
+    let TyIf #_ #_ #_ #_ #t h1 h2 h3 = h in
+    assume (fv_in_env g e1);
+    assume (fv_in_env g e2);
+    assume (fv_in_env g e3);
+    lem_exp_to_fstar g e1 tbool h1;
+    lem_exp_to_fstar g e2 t h2;
+    lem_exp_to_fstar g e3 t h3;
+    let fs_e1 = (exp_to_fstar g e1 tbool h1) in
+    let fs_e2 = (exp_to_fstar g e2 t h2) in
+    let fs_e3 = (exp_to_fstar g e3 t h3) in
+    exp_to_fstar_if g t e1 e2 e3 fs_e1 fs_e2 fs_e3
+  | EFst e12 ->
+    let TyFst #_ #_ #t1 #t2 h1 = h in
+    assume (fv_in_env g e12);
+    lem_exp_to_fstar g e12 (mk_pair t1 t2) h1;
+    let fs_e12 = (exp_to_fstar g e12 (mk_pair t1 t2) h1) in
+    exp_to_fstar_fst g t1 t2 e12 fs_e12  
   | _ -> admit ()
+  | ESnd e12 ->
+    let TySnd #_ #_ #t1 #t2 h1 = h in
+    assume (fv_in_env g e12);
+    lem_exp_to_fstar g e12 (mk_pair t1 t2) h1;
+    let fs_e12 = (exp_to_fstar g e12 (mk_pair t1 t2) h1) in
+    exp_to_fstar_snd g t1 t2 e12 fs_e12
+  | EApp e1 e2 ->
+    let TyApp #_ #_ #_ #t1 #t2 h1 h2 = h in
+    assume (fv_in_env g e1);
+    assume (fv_in_env g e2);
+    lem_exp_to_fstar g e1 (mk_arrow t1 t2) h1;
+    lem_exp_to_fstar g e2 t1 h2;
+    let fs_e1 = (exp_to_fstar g e1 (mk_arrow t1 t2) h1) in
+    let fs_e2 = (exp_to_fstar g e2 t1 h2) in
+    exp_to_fstar_app g t1 t2 e1 e2 fs_e1 fs_e2
+  | ELam body ->
+    let TyLam #_ #body #t1 #t2 hbody = h in
+    assume (fv_in_env (extend t1 g) body);
+    lem_exp_to_fstar (extend t1 g) body t2 hbody;
+    assert (equiv t2 (exp_to_fstar (extend t1 g) body t2 hbody) body);
+    assert (forall b (s:gsub (extend t1 g) b) (fsG:fs_env (extend t1 g)). fsG ∽ s ==> t2 ⦂ ((exp_to_fstar (extend t1 g) body t2 hbody) fsG, gsubst s body)); 
+    let g' = extend t1 g in
+    introduce forall b (s:gsub g b) (fsG:fs_env g). fsG ∽ s ==> (mk_arrow t1 t2) ⦂ ((fun x -> exp_to_fstar (extend t1 g) body t2 hbody (fs_stack fsG x)), gsubst s (ELam body)) with
+      begin
+      let f : (get_Type t1) -> (get_Type t2) = (fun x -> exp_to_fstar (extend t1 g) body t2 hbody (fs_stack fsG x)) in 
+      let body' = subst (sub_elam s) body in
+      assert (gsubst s (ELam body) == ELam body');
+      introduce  fsG ∽ s ==> (mk_arrow t1 t2) ⦂ (f, ELam body') with _. 
+        begin
+        introduce forall (e':closed_exp). steps (ELam body') e' /\ irred e' ==> (mk_arrow t1 t2) ∋ (f, e') with
+          begin
+          assume ((ELam body') == e');
+          introduce _ ==> (mk_arrow t1 t2) ∋ (f, e') with h.
+            begin
+            let RArr #s1 #s2 r1 r2 = get_rel (mk_arrow t1 t2) in
+            introduce forall (v:value) (fs_v:get_Type t1). t1 ∋ (fs_v, v) ==> t2 ⦂ (f fs_v, subst_beta v body') with 
+              begin
+              introduce  t1 ∋ (fs_v, v) ==> _ with _.
+                begin
+                let s' = gsub_extend s t1 v in
+                let fsG' = fs_stack fsG fs_v in
+                lem_substitution s t1 v body;
+                assert (t2 ⦂ (f fs_v, gsubst s' body))
+                end
+              end;
+              assert ((mk_arrow t1 t2) ∋ (f, gsubst s (ELam body)));
+              lem_values_are_expressions (mk_arrow t1 t2) f (gsubst s (ELam body));
+              assert ((mk_arrow t1 t2) ⦂ (f, gsubst s (ELam body))) 
+            end
+          end
+        end
+      end
 
 val lem_bt_ctx i ct : Lemma (
   let (| e, h |) = ct in
